global rename from kevlar to komodo

driver/driver.c
@@ -6,16 +6,16 @@
 #include <linux/cdev.h>
 #include <linux/slab.h>
 #include <linux/highmem.h>
-#include <kevlar/smcapi.h>
-#include "kevdriver.h"
+#include <komodo/smcapi.h>
+#include "driver.h"
 
-MODULE_LICENSE("TBD");
-MODULE_DESCRIPTION("Kevlar driver");
+MODULE_LICENSE("MIT");
+MODULE_DESCRIPTION("Komodo driver");
 
-static dev_t kevlar_dev;
-static struct cdev *kevlar_cdev;
+static dev_t komodo_dev;
+static struct cdev *komodo_cdev;
 
-struct kevlar_client {
+struct komodo_client {
     // TBD
 };
 
@@ -35,12 +35,12 @@ __asm (
 static int test(void)
 {
     int r;
-    kev_err_t err;
+    kom_err_t err;
     u32 addrspace, l1pt, l2pt, disp, code, data;
     struct page *shared_page;
     u32 shared_phys;
     void *shared_virt;
-    kev_multival_t ret;
+    kom_multival_t ret;
 
     shared_page = alloc_page(GFP_KERNEL);
     BUG_ON(shared_page == NULL);
@@ -91,86 +91,86 @@ static int test(void)
            " l2pt %x disp %x code %x data %x\n",
            addrspace, l1pt, l2pt, disp, code, data);
 
-    err = kev_smc_init_addrspace(addrspace, l1pt);
+    err = kom_smc_init_addrspace(addrspace, l1pt);
     printk(KERN_DEBUG "init_addrspace: %d\n", err);
-    if (err != KEV_ERR_SUCCESS) {
+    if (err != KOM_ERR_SUCCESS) {
         return -EIO;
     }
 
-    err = kev_smc_init_dispatcher(disp, addrspace, 0x8000);
+    err = kom_smc_init_dispatcher(disp, addrspace, 0x8000);
     printk(KERN_DEBUG "init_dispatcher: %d\n", err);
-    if (err != KEV_ERR_SUCCESS) {
+    if (err != KOM_ERR_SUCCESS) {
         return -EIO;
     }
 
-    err = kev_smc_init_l2table(l2pt, addrspace, 0);
+    err = kom_smc_init_l2table(l2pt, addrspace, 0);
     printk(KERN_DEBUG "init_l2table: %d\n", err);
-    if (err != KEV_ERR_SUCCESS) {
+    if (err != KOM_ERR_SUCCESS) {
         return -EIO;
     }
 
     /* Populate the page with our test code! */
     memcpy(shared_virt, &test_enclave, &test_enclave_end - &test_enclave);
 
-    err = kev_smc_map_secure(code, addrspace,
-                             0x8000 | KEV_MAPPING_R | KEV_MAPPING_X,
+    err = kom_smc_map_secure(code, addrspace,
+                             0x8000 | KOM_MAPPING_R | KOM_MAPPING_X,
                              shared_phys >> 12);
     printk(KERN_DEBUG "map_secure (code): %d\n", err);
-    if (err != KEV_ERR_SUCCESS) {
+    if (err != KOM_ERR_SUCCESS) {
         return -EIO;
     }
     
-    err = kev_smc_map_secure(data, addrspace,
-                             0x9000 | KEV_MAPPING_R | KEV_MAPPING_W, 0);
+    err = kom_smc_map_secure(data, addrspace,
+                             0x9000 | KOM_MAPPING_R | KOM_MAPPING_W, 0);
     printk(KERN_DEBUG "map_secure (data): %d\n", err);
-    if (err != KEV_ERR_SUCCESS) {
+    if (err != KOM_ERR_SUCCESS) {
         return -EIO;
     }
     
-    err = kev_smc_map_insecure(addrspace, shared_phys >> 12,
-                               0xa000 | KEV_MAPPING_R | KEV_MAPPING_W);
+    err = kom_smc_map_insecure(addrspace, shared_phys >> 12,
+                               0xa000 | KOM_MAPPING_R | KOM_MAPPING_W);
     printk(KERN_DEBUG "map_insecure: %d\n", err);
-    if (err != KEV_ERR_SUCCESS) {
+    if (err != KOM_ERR_SUCCESS) {
         return -EIO;
     }
 
-    err = kev_smc_finalise(addrspace);
+    err = kom_smc_finalise(addrspace);
     printk(KERN_DEBUG "finalise: %d\n", err);
-    if (err != KEV_ERR_SUCCESS) {
+    if (err != KOM_ERR_SUCCESS) {
         return -EIO;
     }
     
-    ret = kev_smc_enter(disp, 1, 2, 3);
+    ret = kom_smc_enter(disp, 1, 2, 3);
     printk(KERN_DEBUG "enter: %d\n", ret.x.err);
-    if (ret.x.err != KEV_ERR_SUCCESS) {
+    if (ret.x.err != KOM_ERR_SUCCESS) {
         return -EIO;
     }
 
     printk(KERN_DEBUG "returned: %lx\n", ret.x.val);
     printk(KERN_DEBUG "wrote: %x\n", *(u32 *)shared_virt);
 
-    err = kev_smc_stop(addrspace);
+    err = kom_smc_stop(addrspace);
     printk(KERN_DEBUG "stop: %d\n", err);
-    if (err != KEV_ERR_SUCCESS) {
+    if (err != KOM_ERR_SUCCESS) {
         return -EIO;
     }
 
-    err = kev_smc_remove(disp);
+    err = kom_smc_remove(disp);
     printk(KERN_DEBUG "remove: %d\n", err);
 
-    err = kev_smc_remove(code);
+    err = kom_smc_remove(code);
     printk(KERN_DEBUG "remove: %d\n", err);
 
-    err = kev_smc_remove(data);
+    err = kom_smc_remove(data);
     printk(KERN_DEBUG "remove: %d\n", err);
 
-    err = kev_smc_remove(l2pt);
+    err = kom_smc_remove(l2pt);
     printk(KERN_DEBUG "remove: %d\n", err);
 
-    err = kev_smc_remove(l1pt);
+    err = kom_smc_remove(l1pt);
     printk(KERN_DEBUG "remove: %d\n", err);
 
-    err = kev_smc_remove(addrspace);
+    err = kom_smc_remove(addrspace);
     printk(KERN_DEBUG "remove: %d\n", err);
 
     kunmap(shared_page);
@@ -179,47 +179,47 @@ static int test(void)
     return 0;
 }
 
-static int kevlar_open(struct inode *inode, struct file *filp)
+static int komodo_open(struct inode *inode, struct file *filp)
 {
-    struct kevlar_client *client = kzalloc(sizeof(*client), GFP_KERNEL);
+    struct komodo_client *client = kzalloc(sizeof(*client), GFP_KERNEL);
 
     filp->private_data = client;
 
     return 0;
 }
 
-static int kevlar_release(struct inode *inode, struct file *filp)
+static int komodo_release(struct inode *inode, struct file *filp)
 {
-    struct kevlar_client *client = filp->private_data;
+    struct komodo_client *client = filp->private_data;
     filp->private_data = NULL; // just for sanity
     kfree(client);
     return 0;
 }
 
-static long kevlar_ioctl(struct file *filp, unsigned int cmd, unsigned long arg)
+static long komodo_ioctl(struct file *filp, unsigned int cmd, unsigned long arg)
 {
     return -ENOTTY;
 }
 
-static struct file_operations kevlar_fops = {
+static struct file_operations komodo_fops = {
     .owner = THIS_MODULE,
-    .open = kevlar_open,
-    .unlocked_ioctl = kevlar_ioctl,
-    .release = kevlar_release,
+    .open = komodo_open,
+    .unlocked_ioctl = komodo_ioctl,
+    .release = komodo_release,
 };
 
 static void driver_exit(void)
 {
-    printk(KERN_INFO "Kevlar driver exiting\n");
+    printk(KERN_INFO "Komodo driver exiting\n");
 
-    if (kevlar_cdev != NULL) {
-        cdev_del(kevlar_cdev);
-        kevlar_cdev = NULL;
+    if (komodo_cdev != NULL) {
+        cdev_del(komodo_cdev);
+        komodo_cdev = NULL;
     }
 
-    if (kevlar_dev != 0) {
-        unregister_chrdev_region(kevlar_dev, 1);
-        kevlar_dev = 0;
+    if (komodo_dev != 0) {
+        unregister_chrdev_region(komodo_dev, 1);
+        komodo_dev = 0;
     }
 
     pgalloc_cleanup();
@@ -230,47 +230,47 @@ static int __init driver_init(void)
     int r;
     u32 magic, npages;
 
-    printk(KERN_INFO "Kevlar driver init\n");
+    printk(KERN_INFO "Komodo driver init\n");
 
-    magic = kev_smc_query();
-    if (magic != KEV_MAGIC) {
-        printk(KERN_ERR "kevlar: query SMC to monitor failed: %x\n", magic);
+    magic = kom_smc_query();
+    if (magic != KOM_MAGIC) {
+        printk(KERN_ERR "komodo: query SMC to monitor failed: %x\n", magic);
         r = -ENODEV;
         goto fail;
     }
 
-    npages = kev_smc_get_phys_pages();
-    printk(KERN_DEBUG "kevlar: %u pages available\n", npages);
+    npages = kom_smc_get_phys_pages();
+    printk(KERN_DEBUG "komodo: %u pages available\n", npages);
 
     r = pgalloc_init(npages);
     if (r != 0) {
-        printk(KERN_ERR "kevlar: pgalloc_init(%u) failed: %x\n", npages, r);
+        printk(KERN_ERR "komodo: pgalloc_init(%u) failed: %x\n", npages, r);
         goto fail;
     }
 
-    printk(KERN_DEBUG "kevlar: running tests\n");
+    printk(KERN_DEBUG "komodo: running tests\n");
     r = test();
-    printk(KERN_DEBUG "kevlar: test complete: %d\n", r);
+    printk(KERN_DEBUG "komodo: test complete: %d\n", r);
     
-    r = alloc_chrdev_region(&kevlar_dev, 0, 1, "kevlar");
+    r = alloc_chrdev_region(&komodo_dev, 0, 1, "komodo");
     if (r != 0) {
-        printk(KERN_ERR "kevlar: alloc_chrdev_region failed: %x\n", r);
+        printk(KERN_ERR "komodo: alloc_chrdev_region failed: %x\n", r);
         goto fail;
     }
 
-    kevlar_cdev = cdev_alloc();
-    if (kevlar_cdev == NULL) {
-        printk(KERN_ERR "kevlar: cdev_alloc failed\n");
+    komodo_cdev = cdev_alloc();
+    if (komodo_cdev == NULL) {
+        printk(KERN_ERR "komodo: cdev_alloc failed\n");
         r = -ENOMEM;
         goto fail;
     }
 
-    kevlar_cdev->owner = THIS_MODULE;
-    kevlar_cdev->ops = &kevlar_fops;
+    komodo_cdev->owner = THIS_MODULE;
+    komodo_cdev->ops = &komodo_fops;
 
-    r = cdev_add(kevlar_cdev, kevlar_dev, 1);
+    r = cdev_add(komodo_cdev, komodo_dev, 1);
     if (r < 0) {
-        printk(KERN_ERR "kevlar: cdev_add failed: %x\n", r);
+        printk(KERN_ERR "komodo: cdev_add failed: %x\n", r);
         goto fail;
     }
 
