driver/smcapi.c
@@ -1,96 +1,96 @@
 #include <linux/kernel.h>
-#include <kevlar/smcapi.h>
+#include <komodo/smcapi.h>
 
 asmlinkage u64 invoke_smc(u32 callno, u32 arg1, u32 arg2, u32 arg3, u32 arg4);
 
-uint32_t kev_smc_query(void)
+uint32_t kom_smc_query(void)
 {
-    kev_multival_t ret;
-    ret.raw = invoke_smc(KEV_SMC_QUERY,0,0,0,0);
+    kom_multival_t ret;
+    ret.raw = invoke_smc(KOM_SMC_QUERY,0,0,0,0);
     return ret.x.err;
 }
 
-uint32_t kev_smc_get_phys_pages(void)
+uint32_t kom_smc_get_phys_pages(void)
 {
-    kev_multival_t ret;
-    ret.raw = invoke_smc(KEV_SMC_GETPHYSPAGES,0,0,0,0);
-    BUG_ON(ret.x.err != KEV_ERR_SUCCESS);
+    kom_multival_t ret;
+    ret.raw = invoke_smc(KOM_SMC_GETPHYSPAGES,0,0,0,0);
+    BUG_ON(ret.x.err != KOM_ERR_SUCCESS);
     return ret.x.val;
 }
 
-kev_err_t kev_smc_init_addrspace(kev_secure_pageno_t addrspace_page,
-                                 kev_secure_pageno_t l1pt_page)
+kom_err_t kom_smc_init_addrspace(kom_secure_pageno_t addrspace_page,
+                                 kom_secure_pageno_t l1pt_page)
 {
-    kev_multival_t ret;
-    ret.raw = invoke_smc(KEV_SMC_INIT_ADDRSPACE, addrspace_page, l1pt_page, 0, 0);
+    kom_multival_t ret;
+    ret.raw = invoke_smc(KOM_SMC_INIT_ADDRSPACE, addrspace_page, l1pt_page, 0, 0);
     return ret.x.err;
 }
 
-kev_err_t kev_smc_init_dispatcher(kev_secure_pageno_t page,
-                                  kev_secure_pageno_t addrspace,
+kom_err_t kom_smc_init_dispatcher(kom_secure_pageno_t page,
+                                  kom_secure_pageno_t addrspace,
                                   uint32_t entrypoint)
 {
-    kev_multival_t ret;
-    ret.raw = invoke_smc(KEV_SMC_INIT_DISPATCHER, page, addrspace, entrypoint, 0);
+    kom_multival_t ret;
+    ret.raw = invoke_smc(KOM_SMC_INIT_DISPATCHER, page, addrspace, entrypoint, 0);
     return ret.x.err;
 }
 
-kev_err_t kev_smc_init_l2table(kev_secure_pageno_t page,
-                               kev_secure_pageno_t addrspace,
+kom_err_t kom_smc_init_l2table(kom_secure_pageno_t page,
+                               kom_secure_pageno_t addrspace,
                                uint32_t l1_index)
 {
-    kev_multival_t ret;
-    ret.raw = invoke_smc(KEV_SMC_INIT_L2PTABLE, page, addrspace, l1_index, 0);
+    kom_multival_t ret;
+    ret.raw = invoke_smc(KOM_SMC_INIT_L2PTABLE, page, addrspace, l1_index, 0);
     return ret.x.err;
 }
 
-kev_err_t kev_smc_map_secure(kev_secure_pageno_t page,
-                             kev_secure_pageno_t addrspace,
+kom_err_t kom_smc_map_secure(kom_secure_pageno_t page,
+                             kom_secure_pageno_t addrspace,
                              uint32_t mapping,
                              uint32_t phys_pageno)
 {
-    kev_multival_t ret;
-    ret.raw = invoke_smc(KEV_SMC_MAP_SECURE, page, addrspace, mapping, phys_pageno);
+    kom_multival_t ret;
+    ret.raw = invoke_smc(KOM_SMC_MAP_SECURE, page, addrspace, mapping, phys_pageno);
     return ret.x.err;
 }
 
-kev_err_t kev_smc_map_insecure(kev_secure_pageno_t addrspace,
+kom_err_t kom_smc_map_insecure(kom_secure_pageno_t addrspace,
                                uint32_t phys_pageno,
                                uint32_t mapping)
 {
-    kev_multival_t ret;
-    ret.raw = invoke_smc(KEV_SMC_MAP_INSECURE, addrspace, phys_pageno, mapping, 0);
+    kom_multival_t ret;
+    ret.raw = invoke_smc(KOM_SMC_MAP_INSECURE, addrspace, phys_pageno, mapping, 0);
     return ret.x.err;
 }
 
-kev_err_t kev_smc_remove(kev_secure_pageno_t page)
+kom_err_t kom_smc_remove(kom_secure_pageno_t page)
 {
-    kev_multival_t ret;
-    ret.raw = invoke_smc(KEV_SMC_REMOVE, page, 0, 0, 0);
+    kom_multival_t ret;
+    ret.raw = invoke_smc(KOM_SMC_REMOVE, page, 0, 0, 0);
     return ret.x.err;
 }
 
-kev_err_t kev_smc_finalise(kev_secure_pageno_t addrspace)
+kom_err_t kom_smc_finalise(kom_secure_pageno_t addrspace)
 {
-    kev_multival_t ret;
-    ret.raw = invoke_smc(KEV_SMC_FINALISE, addrspace, 0, 0, 0);
+    kom_multival_t ret;
+    ret.raw = invoke_smc(KOM_SMC_FINALISE, addrspace, 0, 0, 0);
     return ret.x.err;
 }
 
-kev_err_t kev_smc_stop(kev_secure_pageno_t addrspace)
+kom_err_t kom_smc_stop(kom_secure_pageno_t addrspace)
 {
-    kev_multival_t ret;
-    ret.raw = invoke_smc(KEV_SMC_STOP, addrspace, 0, 0, 0);
+    kom_multival_t ret;
+    ret.raw = invoke_smc(KOM_SMC_STOP, addrspace, 0, 0, 0);
     return ret.x.err;
 }
 
-kev_multival_t kev_smc_enter(kev_secure_pageno_t dispatcher, uintptr_t arg1,
+kom_multival_t kom_smc_enter(kom_secure_pageno_t dispatcher, uintptr_t arg1,
                              uintptr_t arg2, uintptr_t arg3)
 {
-    kev_multival_t ret;
-    ret.raw = invoke_smc(KEV_SMC_ENTER, dispatcher, arg1, arg2, arg3);
-    while (ret.x.err == KEV_ERR_INTERRUPTED) {
-        ret.raw = invoke_smc(KEV_SMC_RESUME, dispatcher, 0, 0, 0);
+    kom_multival_t ret;
+    ret.raw = invoke_smc(KOM_SMC_ENTER, dispatcher, arg1, arg2, arg3);
+    while (ret.x.err == KOM_ERR_INTERRUPTED) {
+        ret.raw = invoke_smc(KOM_SMC_RESUME, dispatcher, 0, 0, 0);
     }
 
     return ret;
