include/komodo/memregions.h
@@ -1,7 +1,7 @@
-#ifndef KEVLAR_MEMREGIONS_H
-#define KEVLAR_MEMREGIONS_H
+#ifndef KOM_MEMREGIONS_H
+#define KOM_MEMREGIONS_H
 
-/* Kevlar secure world virtual address map:
+/* Komodo secure world virtual address map:
  *
  * 0-1GB "User-mode" portion of the address map, used only for enclaves.
  *       This is mapped by a 4kB root page table in TTBR0.
@@ -18,18 +18,18 @@
  * plus unsecure pages for I/O with normal world.)
  */
 
-#define KEVLAR_PAGE_SIZE        0x1000
+#define KOM_PAGE_SIZE        0x1000
 
 // user/kernel split for secure world
-#define KEVLAR_MON_VBASE        ((uintptr_t)0x40000000)
+#define KOM_MON_VBASE        ((uintptr_t)0x40000000)
 
 // virtual mapping of monitor's direct view of _all_ RAM
 // (obviously this only works for rather small RAM sizes! :)
-#define KEVLAR_DIRECTMAP_VBASE  ((uintptr_t)0x80000000)
-#define KEVLAR_DIRECTMAP_SIZE   ((uintptr_t)0x80000000)
+#define KOM_DIRECTMAP_VBASE  ((uintptr_t)0x80000000)
+#define KOM_DIRECTMAP_SIZE   ((uintptr_t)0x80000000)
 
 // number of supported secure pages
-#define KEVLAR_SECURE_RESERVE   (1 * 1024 * 1024)
-#define KEVLAR_SECURE_NPAGES    (KEVLAR_SECURE_RESERVE / KEVLAR_PAGE_SIZE)
+#define KOM_SECURE_RESERVE   (1 * 1024 * 1024)
+#define KOM_SECURE_NPAGES    (KOM_SECURE_RESERVE / KOM_PAGE_SIZE)
 
 #endif
