include/komodo/smcapi.h
@@ -1,0 +1,98 @@
+#ifndef _KOM_SMCAPI_H
+#define _KOM_SMCAPI_H
+
+#define KOM_SMC_QUERY           1
+#define KOM_SMC_GETPHYSPAGES    2
+#define KOM_SMC_INIT_ADDRSPACE  10
+#define KOM_SMC_INIT_DISPATCHER 11
+#define KOM_SMC_INIT_L2PTABLE   12
+#define KOM_SMC_MAP_SECURE      13
+#define KOM_SMC_MAP_INSECURE    14
+#define KOM_SMC_REMOVE          20
+#define KOM_SMC_FINALISE        21
+#define KOM_SMC_ENTER           22
+#define KOM_SMC_RESUME          23
+#define KOM_SMC_STOP            29
+
+#define KOM_MAGIC 0x4b6d646f // "Kmdo"
+
+typedef uint32_t kom_err_t;
+typedef uint32_t kom_secure_pageno_t;
+
+#define KOM_ERR_SUCCESS         0
+#define KOM_ERR_INVALID_PAGENO  1
+#define KOM_ERR_PAGEINUSE       2
+#define KOM_ERR_INVALID_ADDRSPACE 3
+#define KOM_ERR_ALREADY_FINAL   4
+#define KOM_ERR_NOT_FINAL       5
+#define KOM_ERR_INVALID_MAPPING 6
+#define KOM_ERR_ADDRINUSE       7
+#define KOM_ERR_NOT_STOPPED     8
+#define KOM_ERR_INTERRUPTED     9
+#define KOM_ERR_FAULT           10
+#define KOM_ERR_ALREADY_ENTERED 11
+#define KOM_ERR_NOT_ENTERED     12
+#define KOM_ERR_INVALID         ((kom_err_t)-1)
+
+// struct type for returning two values across an SMC API
+typedef union kom_multival {
+    uint64_t raw;
+    struct {
+        kom_err_t err;
+        uintptr_t val;
+    } x;
+} kom_multival_t;
+
+// returns KVR_MAGIC
+uint32_t kom_smc_query(void);
+
+// return number of secure pages
+uint32_t kom_smc_get_phys_pages(void);
+
+kom_err_t kom_smc_init_addrspace(kom_secure_pageno_t addrspace_page,
+                                 kom_secure_pageno_t l1pt_page);
+
+kom_err_t kom_smc_init_dispatcher(kom_secure_pageno_t page,
+                                  kom_secure_pageno_t addrspace,
+                                  uint32_t entrypoint);
+
+kom_err_t kom_smc_init_l2table(kom_secure_pageno_t page,
+                               kom_secure_pageno_t addrspace,
+                               uint32_t l1_index);
+
+// calls to establish a page mapping (secure or insecure) use the following
+// simple format: the low three bits identify the permissions
+#define KOM_MAPPING_R   1
+#define KOM_MAPPING_W   2
+#define KOM_MAPPING_X   4
+
+// the virtual page number is shifted 12 bits to the left, i.e. where
+// you would expect :), so that the MSB of the 4K page number is the
+// MSB of the 32-bit address
+#define KOM_MAPPING_VPAGENO_SHIFT 12
+
+// other bits in the mapping word are presently reserved
+#define KOM_MAPPING_RESERVED_MASK 0xff7
+
+// map a secure page
+kom_err_t kom_smc_map_secure(kom_secure_pageno_t page,
+                             kom_secure_pageno_t addrspace,
+                             uint32_t mapping,
+                             uint32_t phys_pageno);
+
+// map any other (non-secure) physical page
+kom_err_t kom_smc_map_insecure(kom_secure_pageno_t addrspace,
+                               uint32_t phys_pageno,
+                               uint32_t mapping);
+
+// remove this page from its address space, or reclaim the address space (only possible once stopped)
+kom_err_t kom_smc_remove(kom_secure_pageno_t page);
+
+kom_err_t kom_smc_finalise(kom_secure_pageno_t addrspace);
+kom_err_t kom_smc_stop(kom_secure_pageno_t addrspace);
+
+kom_multival_t kom_smc_enter(kom_secure_pageno_t dispatcher, uintptr_t arg1,
+                             uintptr_t arg2, uintptr_t arg3);
+kom_multival_t kom_smc_resume(kom_secure_pageno_t dispatcher);
+
+#endif
