monitor/monitor.c
@@ -1,45 +1,43 @@
 #include <stdint.h>
 #include <string.h>
-#include <kevlar/memregions.h>
-#include <kevlar/smcapi.h>
 #include "monitor.h"
 
 #define ARM_SCR_FIQ     0x04 // FIQ handler monitor mode
 #define ARM_SCR_IRQ     0x02 // IRQ handler monitor mode
 #define ARM_SCR_NS      0x01 // non-secure bit
 
-static struct kev_pagedb_entry g_pagedb[KEVLAR_SECURE_NPAGES];
+static struct kom_pagedb_entry g_pagedb[KOM_SECURE_NPAGES];
 uintptr_t g_secure_physbase;
-static struct kev_addrspace *g_cur_addrspace;
-struct kev_dispatcher *g_cur_dispatcher;
+static struct kom_addrspace *g_cur_addrspace;
+struct kom_dispatcher *g_cur_dispatcher;
 
-static inline bool page_is_valid(kev_secure_pageno_t pageno)
+static inline bool page_is_valid(kom_secure_pageno_t pageno)
 {
-    return pageno < KEVLAR_SECURE_NPAGES;
+    return pageno < KOM_SECURE_NPAGES;
 }
 
-static inline bool page_is_typed(kev_secure_pageno_t pageno, kev_pagetype_t type)
+static inline bool page_is_typed(kom_secure_pageno_t pageno, kom_pagetype_t type)
 {
     return page_is_valid(pageno) && g_pagedb[pageno].type == type;
 }
 
-static inline bool page_is_free(kev_secure_pageno_t pageno)
+static inline bool page_is_free(kom_secure_pageno_t pageno)
 {
-    return page_is_typed(pageno, KEV_PAGE_FREE);
+    return page_is_typed(pageno, KOM_PAGE_FREE);
 }
 
-static inline uintptr_t page_paddr(kev_secure_pageno_t pageno)
+static inline uintptr_t page_paddr(kom_secure_pageno_t pageno)
 {
     //assert(page_is_valid(pageno));
-    return g_secure_physbase + pageno * KEVLAR_PAGE_SIZE;
+    return g_secure_physbase + pageno * KOM_PAGE_SIZE;
 }
 
 static inline void *phys2monvaddr(uintptr_t phys)
 {
-    return (void *)(phys + KEVLAR_DIRECTMAP_VBASE);
+    return (void *)(phys + KOM_DIRECTMAP_VBASE);
 }
 
-static inline void *page_monvaddr(kev_secure_pageno_t pageno)
+static inline void *page_monvaddr(kom_secure_pageno_t pageno)
 {
     return phys2monvaddr(page_paddr(pageno));
 }
@@ -101,7 +99,7 @@ static void leave_secure_world(void)
     __asm volatile("msr lr_und, %0" :: "r" (lr_und));
 }
 
-static void switch_addrspace(struct kev_addrspace *addrspace)
+static void switch_addrspace(struct kom_addrspace *addrspace)
 {
     if (g_cur_addrspace == addrspace) {
         return;
@@ -130,126 +128,126 @@ static void switch_addrspace(struct kev_addrspace *addrspace)
     g_cur_addrspace = addrspace;
 }
 
-static kev_err_t allocate_page(kev_secure_pageno_t page,
-                               struct kev_addrspace *addrspace,
-                               kev_pagetype_t type)
+static kom_err_t allocate_page(kom_secure_pageno_t page,
+                               struct kom_addrspace *addrspace,
+                               kom_pagetype_t type)
 {
     if (!page_is_valid(page)) {
-        return KEV_ERR_INVALID_PAGENO;
+        return KOM_ERR_INVALID_PAGENO;
     }
 
     if (!page_is_free(page)) {
-        return KEV_ERR_PAGEINUSE;
+        return KOM_ERR_PAGEINUSE;
     }
 
-    if (addrspace->state != KEV_ADDRSPACE_INIT) {
-        return KEV_ERR_ALREADY_FINAL;
+    if (addrspace->state != KOM_ADDRSPACE_INIT) {
+        return KOM_ERR_ALREADY_FINAL;
     }
 
-    if (type != KEV_PAGE_DATA) {
-        memset(page_monvaddr(page), 0, KEVLAR_PAGE_SIZE);
+    if (type != KOM_PAGE_DATA) {
+        memset(page_monvaddr(page), 0, KOM_PAGE_SIZE);
     }
 
     g_pagedb[page].type = type;
     g_pagedb[page].addrspace = addrspace;
     addrspace->refcount++;
 
-    return KEV_ERR_SUCCESS;
+    return KOM_ERR_SUCCESS;
 }
 
-static struct kev_addrspace *get_addrspace(kev_secure_pageno_t page)
+static struct kom_addrspace *get_addrspace(kom_secure_pageno_t page)
 {
-    if (page_is_typed(page, KEV_PAGE_ADDRSPACE)) {
+    if (page_is_typed(page, KOM_PAGE_ADDRSPACE)) {
         return page_monvaddr(page);
     } else {
         return NULL;
     }    
 }
 
-uint32_t kev_smc_get_phys_pages(void)
+uint32_t kom_smc_get_phys_pages(void)
 {
-    return KEVLAR_SECURE_NPAGES;
+    return KOM_SECURE_NPAGES;
 }
 
-kev_err_t kev_smc_init_addrspace(kev_secure_pageno_t addrspace_page,
-                                 kev_secure_pageno_t l1pt_page)
+kom_err_t kom_smc_init_addrspace(kom_secure_pageno_t addrspace_page,
+                                 kom_secure_pageno_t l1pt_page)
 {
     if (addrspace_page == l1pt_page
         || !(page_is_valid(addrspace_page) && page_is_valid(l1pt_page))) {
-        return KEV_ERR_INVALID_PAGENO;
+        return KOM_ERR_INVALID_PAGENO;
     }
 
     // ARM requires that the level 1 page table be 16kB-aligned
     // (even though our use of TTBCR only requires it to be 4kB in size)
     if (l1pt_page % 4 != 0) {
-        return KEV_ERR_INVALID_PAGENO;
+        return KOM_ERR_INVALID_PAGENO;
     }
 
     if (!(page_is_free(addrspace_page) && page_is_free(l1pt_page))) {
-        return KEV_ERR_PAGEINUSE;
+        return KOM_ERR_PAGEINUSE;
     }
 
-    struct kev_addrspace *addrspace = page_monvaddr(addrspace_page);
+    struct kom_addrspace *addrspace = page_monvaddr(addrspace_page);
 
-    memset(addrspace, 0, KEVLAR_PAGE_SIZE);
-    memset(page_monvaddr(l1pt_page), 0, KEVLAR_PAGE_SIZE);
+    memset(addrspace, 0, KOM_PAGE_SIZE);
+    memset(page_monvaddr(l1pt_page), 0, KOM_PAGE_SIZE);
 
-    g_pagedb[addrspace_page].type = KEV_PAGE_ADDRSPACE;
+    g_pagedb[addrspace_page].type = KOM_PAGE_ADDRSPACE;
     g_pagedb[addrspace_page].addrspace = addrspace;
-    g_pagedb[l1pt_page].type = KEV_PAGE_L1PTABLE;
+    g_pagedb[l1pt_page].type = KOM_PAGE_L1PTABLE;
     g_pagedb[l1pt_page].addrspace = addrspace;
 
     addrspace->l1pt = page_monvaddr(l1pt_page);
     addrspace->l1pt_phys = page_paddr(l1pt_page);
     addrspace->refcount = 1; // for the l1pt
-    addrspace->state = KEV_ADDRSPACE_INIT;
+    addrspace->state = KOM_ADDRSPACE_INIT;
 
-    return KEV_ERR_SUCCESS;
+    return KOM_ERR_SUCCESS;
 }
 
-kev_err_t kev_smc_init_dispatcher(kev_secure_pageno_t page,
-                                  kev_secure_pageno_t addrspace_page,
+kom_err_t kom_smc_init_dispatcher(kom_secure_pageno_t page,
+                                  kom_secure_pageno_t addrspace_page,
                                   uint32_t entrypoint)
 {
-    kev_err_t err;
+    kom_err_t err;
 
-    struct kev_addrspace *addrspace = get_addrspace(addrspace_page);
+    struct kom_addrspace *addrspace = get_addrspace(addrspace_page);
     if (addrspace == NULL) {
-        return KEV_ERR_INVALID_ADDRSPACE;
+        return KOM_ERR_INVALID_ADDRSPACE;
     }
 
-    err = allocate_page(page, addrspace, KEV_PAGE_DISPATCHER);
-    if (err != KEV_ERR_SUCCESS) {
+    err = allocate_page(page, addrspace, KOM_PAGE_DISPATCHER);
+    if (err != KOM_ERR_SUCCESS) {
         return err;
     }
 
-    struct kev_dispatcher *disp = page_monvaddr(page);
+    struct kom_dispatcher *disp = page_monvaddr(page);
     disp->entrypoint = entrypoint;
 
-    return KEV_ERR_SUCCESS;
+    return KOM_ERR_SUCCESS;
 }
 
-kev_err_t kev_smc_init_l2table(kev_secure_pageno_t page,
-                               kev_secure_pageno_t addrspace_page,
+kom_err_t kom_smc_init_l2table(kom_secure_pageno_t page,
+                               kom_secure_pageno_t addrspace_page,
                                uint32_t l1_index)
 {
-    kev_err_t err;
+    kom_err_t err;
 
     if (l1_index >= 256) {
-        return KEV_ERR_INVALID_MAPPING;
+        return KOM_ERR_INVALID_MAPPING;
     }
 
-    struct kev_addrspace *addrspace = get_addrspace(addrspace_page);
+    struct kom_addrspace *addrspace = get_addrspace(addrspace_page);
     if (addrspace == NULL) {
-        return KEV_ERR_INVALID_ADDRSPACE;
+        return KOM_ERR_INVALID_ADDRSPACE;
     }
 
     if (addrspace->l1pt[l1_index].raw != 0) {
-        return KEV_ERR_ADDRINUSE;
+        return KOM_ERR_ADDRINUSE;
     }
 
-    err = allocate_page(page, addrspace, KEV_PAGE_L2PTABLE);
-    if (err != KEV_ERR_SUCCESS) {
+    err = allocate_page(page, addrspace, KOM_PAGE_L2PTABLE);
+    if (err != KOM_ERR_SUCCESS) {
         return err;
     }
 
@@ -274,10 +272,10 @@ kev_err_t kev_smc_init_l2table(kev_secure_pageno_t page,
     pte.pagetable.ptbase++;
     addrspace->l1pt[l1_index * 4 + 3].raw = pte.raw;
 
-    return KEV_ERR_SUCCESS;
+    return KOM_ERR_SUCCESS;
 }
 
-static armpte_short_l2 *lookup_pte(struct kev_addrspace *addrspace,
+static armpte_short_l2 *lookup_pte(struct kom_addrspace *addrspace,
                                    uint32_t mapping)
 {
     // check that it's within the addressable region
@@ -297,28 +295,28 @@ static armpte_short_l2 *lookup_pte(struct kev_addrspace *addrspace,
     return &l2pt[l2index];
 }
 
-static kev_err_t is_valid_mapping_target(struct kev_addrspace *addrspace,
+static kom_err_t is_valid_mapping_target(struct kom_addrspace *addrspace,
                                          uint32_t mapping)
 {
-    if (addrspace->state != KEV_ADDRSPACE_INIT) {
-        return KEV_ERR_ALREADY_FINAL;
+    if (addrspace->state != KOM_ADDRSPACE_INIT) {
+        return KOM_ERR_ALREADY_FINAL;
     }
 
     // check for a supported combination of permissions: RO, RW, RX, RWX
-    if (!(mapping & KEV_MAPPING_R)) {
-        return KEV_ERR_INVALID_MAPPING;
+    if (!(mapping & KOM_MAPPING_R)) {
+        return KOM_ERR_INVALID_MAPPING;
     }
 
     // check that the target address is mappable and free
     armpte_short_l2 *l2pte = lookup_pte(addrspace, mapping);
     if (l2pte == NULL || l2pte->invalid.type != 0) {
-        return KEV_ERR_INVALID_MAPPING;
+        return KOM_ERR_INVALID_MAPPING;
     }
 
-    return KEV_ERR_SUCCESS;
+    return KOM_ERR_SUCCESS;
 }
 
-static void map_page(struct kev_addrspace *addrspace, uint32_t mapping,
+static void map_page(struct kom_addrspace *addrspace, uint32_t mapping,
                      uintptr_t paddr)
 {
     armpte_short_l2 *pte = lookup_pte(addrspace, mapping);
@@ -326,14 +324,14 @@ static void map_page(struct kev_addrspace *addrspace, uint32_t mapping,
 
     pte->raw = (armpte_short_l2) {
         .smallpage = {
-            .xn = !(mapping & KEV_MAPPING_X),
+            .xn = !(mapping & KOM_MAPPING_X),
             .type = 1,
             .b = 1, // write-back, write-allocate
             .c = 0, // write-back, write-allocate
             .ap0 = 1, // access flag = 1 (already accessed)
             .ap1 = 1, // user
             .tex = 5, // 0b101: cacheable, write-back, write-allocate
-            .ap2 = !(mapping & KEV_MAPPING_W),
+            .ap2 = !(mapping & KOM_MAPPING_W),
             .s = 1, // shareable
             .ng = 1, // not global; TODO: ASID management!
             .base = paddr >> 12
@@ -344,9 +342,9 @@ static void map_page(struct kev_addrspace *addrspace, uint32_t mapping,
 // is the given physical (0-based) page number located in our secure region?
 static bool phys_page_is_secure(uintptr_t phys_pageno)
 {
-    uintptr_t paddr = phys_pageno * KEVLAR_PAGE_SIZE;
+    uintptr_t paddr = phys_pageno * KOM_PAGE_SIZE;
     return paddr >= g_secure_physbase
-        && paddr < g_secure_physbase + page_paddr(KEVLAR_SECURE_NPAGES);
+        && paddr < g_secure_physbase + page_paddr(KOM_SECURE_NPAGES);
 }
 
 // is the given physical (0-based) page number located in memory, so
@@ -354,35 +352,35 @@ static bool phys_page_is_secure(uintptr_t phys_pageno)
 static bool phys_page_is_ram(uintptr_t phys_pageno)
 {
     // XXX: this is a pi-specific assumption
-    return phys_pageno * KEVLAR_PAGE_SIZE < g_secure_physbase;
+    return phys_pageno * KOM_PAGE_SIZE < g_secure_physbase;
 }
 
-kev_err_t kev_smc_map_secure(kev_secure_pageno_t page,
-                             kev_secure_pageno_t addrspace_page,
+kom_err_t kom_smc_map_secure(kom_secure_pageno_t page,
+                             kom_secure_pageno_t addrspace_page,
                              uint32_t mapping,
                              uint32_t phys_pageno)
 {
-    kev_err_t err;
+    kom_err_t err;
 
-    struct kev_addrspace *addrspace = get_addrspace(addrspace_page);
+    struct kom_addrspace *addrspace = get_addrspace(addrspace_page);
     if (addrspace == NULL) {
-        return KEV_ERR_INVALID_ADDRSPACE;
+        return KOM_ERR_INVALID_ADDRSPACE;
     }
 
     err = is_valid_mapping_target(addrspace, mapping);
-    if (err != KEV_ERR_SUCCESS) {
+    if (err != KOM_ERR_SUCCESS) {
         return err;
     }
 
     // check the validity initial page we are being asked to copy
     if (phys_pageno != 0 &&
         !(phys_page_is_ram(phys_pageno) && !phys_page_is_secure(phys_pageno))) {
-        return KEV_ERR_INVALID_PAGENO;
+        return KOM_ERR_INVALID_PAGENO;
     }
 
     // allocate the page
-    err = allocate_page(page, addrspace, KEV_PAGE_DATA);
-    if (err != KEV_ERR_SUCCESS) {
+    err = allocate_page(page, addrspace, KOM_PAGE_DATA);
+    if (err != KOM_ERR_SUCCESS) {
         return err;
     }
 
@@ -390,65 +388,65 @@ kev_err_t kev_smc_map_secure(kev_secure_pageno_t page,
 
     // initialise it
     if (phys_pageno == 0) {
-        memset(page_monvaddr(page), 0, KEVLAR_PAGE_SIZE);
+        memset(page_monvaddr(page), 0, KOM_PAGE_SIZE);
     } else {
         memcpy(page_monvaddr(page),
-               phys2monvaddr(phys_pageno * KEVLAR_PAGE_SIZE),
-               KEVLAR_PAGE_SIZE);
+               phys2monvaddr(phys_pageno * KOM_PAGE_SIZE),
+               KOM_PAGE_SIZE);
     }
 
     map_page(addrspace, mapping, page_paddr(page));
 
-    return KEV_ERR_SUCCESS;
+    return KOM_ERR_SUCCESS;
 }
 
-kev_err_t kev_smc_map_insecure(kev_secure_pageno_t addrspace_page,
+kom_err_t kom_smc_map_insecure(kom_secure_pageno_t addrspace_page,
                                uint32_t phys_pageno,
                                uint32_t mapping)
 {
-    kev_err_t err;
+    kom_err_t err;
 
-    struct kev_addrspace *addrspace = get_addrspace(addrspace_page);
+    struct kom_addrspace *addrspace = get_addrspace(addrspace_page);
     if (addrspace == NULL) {
-        return KEV_ERR_INVALID_ADDRSPACE;
+        return KOM_ERR_INVALID_ADDRSPACE;
     }
 
     err = is_valid_mapping_target(addrspace, mapping);
-    if (err != KEV_ERR_SUCCESS) {
+    if (err != KOM_ERR_SUCCESS) {
         return err;
     }
 
     // check that the page is not located in our secure region
     if (phys_page_is_secure(phys_pageno)) {
-        return KEV_ERR_INVALID_PAGENO;
+        return KOM_ERR_INVALID_PAGENO;
     }
 
-    map_page(addrspace, mapping, phys_pageno * KEVLAR_PAGE_SIZE);
+    map_page(addrspace, mapping, phys_pageno * KOM_PAGE_SIZE);
 
-    return KEV_ERR_SUCCESS;
+    return KOM_ERR_SUCCESS;
 }
 
-kev_err_t kev_smc_remove(kev_secure_pageno_t pageno)
+kom_err_t kom_smc_remove(kom_secure_pageno_t pageno)
 {
-    struct kev_addrspace *addrspace;
+    struct kom_addrspace *addrspace;
 
     if (!page_is_valid(pageno)) {
-        return KEV_ERR_INVALID_PAGENO;
+        return KOM_ERR_INVALID_PAGENO;
     }
 
-    if (g_pagedb[pageno].type == KEV_PAGE_FREE) {
-        return KEV_ERR_SUCCESS;
+    if (g_pagedb[pageno].type == KOM_PAGE_FREE) {
+        return KOM_ERR_SUCCESS;
     }
 
-    if (g_pagedb[pageno].type == KEV_PAGE_ADDRSPACE) {
+    if (g_pagedb[pageno].type == KOM_PAGE_ADDRSPACE) {
         addrspace = page_monvaddr(pageno);
         if (addrspace->refcount != 0) {
-            return KEV_ERR_PAGEINUSE;
+            return KOM_ERR_PAGEINUSE;
         }
     } else {
         addrspace = g_pagedb[pageno].addrspace;
-        if (addrspace->state != KEV_ADDRSPACE_STOPPED) {
-            return KEV_ERR_NOT_STOPPED;
+        if (addrspace->state != KOM_ADDRSPACE_STOPPED) {
+            return KOM_ERR_NOT_STOPPED;
         }
         addrspace->refcount--;
     }
@@ -457,32 +455,32 @@ kev_err_t kev_smc_remove(kev_secure_pageno_t pageno)
      * addrspace is stopped it can never execute again, so we can just
      * wait for them to be deleted */
 
-    g_pagedb[pageno].type = KEV_PAGE_FREE;
+    g_pagedb[pageno].type = KOM_PAGE_FREE;
     g_pagedb[pageno].addrspace = NULL;
 
-    return KEV_ERR_SUCCESS;
+    return KOM_ERR_SUCCESS;
 }
 
-kev_err_t kev_smc_finalise(kev_secure_pageno_t addrspace_page)
+kom_err_t kom_smc_finalise(kom_secure_pageno_t addrspace_page)
 {
-    struct kev_addrspace *addrspace = get_addrspace(addrspace_page);
+    struct kom_addrspace *addrspace = get_addrspace(addrspace_page);
     if (addrspace == NULL) {
-        return KEV_ERR_INVALID_ADDRSPACE;
+        return KOM_ERR_INVALID_ADDRSPACE;
     }
 
-    if (addrspace->state != KEV_ADDRSPACE_INIT) {
-        return KEV_ERR_ALREADY_FINAL;
+    if (addrspace->state != KOM_ADDRSPACE_INIT) {
+        return KOM_ERR_ALREADY_FINAL;
     }
 
-    addrspace->state = KEV_ADDRSPACE_FINAL;
-    return KEV_ERR_SUCCESS;
+    addrspace->state = KOM_ADDRSPACE_FINAL;
+    return KOM_ERR_SUCCESS;
 }
 
-kev_err_t kev_smc_stop(kev_secure_pageno_t addrspace_page)
+kom_err_t kom_smc_stop(kom_secure_pageno_t addrspace_page)
 {
-    struct kev_addrspace *addrspace = get_addrspace(addrspace_page);
+    struct kom_addrspace *addrspace = get_addrspace(addrspace_page);
     if (addrspace == NULL) {
-        return KEV_ERR_INVALID_ADDRSPACE;
+        return KOM_ERR_INVALID_ADDRSPACE;
     }
 
     if (g_cur_addrspace == addrspace) {
@@ -491,33 +489,33 @@ kev_err_t kev_smc_stop(kev_secure_pageno_t addrspace_page)
         leave_secure_world();
     }
 
-    addrspace->state = KEV_ADDRSPACE_STOPPED;
+    addrspace->state = KOM_ADDRSPACE_STOPPED;
 
-    return KEV_ERR_SUCCESS;
+    return KOM_ERR_SUCCESS;
 }
 
-kev_multival_t kev_smc_enter(kev_secure_pageno_t disp_page, uintptr_t arg1,
+kom_multival_t kom_smc_enter(kom_secure_pageno_t disp_page, uintptr_t arg1,
                              uintptr_t arg2, uintptr_t arg3)
 {
-    kev_multival_t ret;
+    kom_multival_t ret;
 
     ret.x.val = 0;
     
-    if (!page_is_typed(disp_page, KEV_PAGE_DISPATCHER)) {
-        ret.x.err = KEV_ERR_INVALID_PAGENO;
+    if (!page_is_typed(disp_page, KOM_PAGE_DISPATCHER)) {
+        ret.x.err = KOM_ERR_INVALID_PAGENO;
         return ret;
     }
 
-    struct kev_dispatcher *dispatcher = page_monvaddr(disp_page);
-    struct kev_addrspace *addrspace = g_pagedb[disp_page].addrspace;
+    struct kom_dispatcher *dispatcher = page_monvaddr(disp_page);
+    struct kom_addrspace *addrspace = g_pagedb[disp_page].addrspace;
 
-    if (addrspace->state != KEV_ADDRSPACE_FINAL) {
-        ret.x.err = KEV_ERR_NOT_FINAL;
+    if (addrspace->state != KOM_ADDRSPACE_FINAL) {
+        ret.x.err = KOM_ERR_NOT_FINAL;
         return ret;
     }
 
     if (dispatcher->entered) {
-        ret.x.err = KEV_ERR_ALREADY_ENTERED;
+        ret.x.err = KOM_ERR_ALREADY_ENTERED;
         return ret;
     }
 
@@ -537,7 +535,7 @@ kev_multival_t kev_smc_enter(kev_secure_pageno_t disp_page, uintptr_t arg1,
     g_cur_dispatcher = dispatcher;
     ret.raw = dispatch(dispatcher);
     leave_secure_world();
-    if (ret.x.err == KEV_ERR_INTERRUPTED || ret.x.err == KEV_ERR_FAULT) {
+    if (ret.x.err == KOM_ERR_INTERRUPTED || ret.x.err == KOM_ERR_FAULT) {
         dispatcher->entered = true;
     }
     g_cur_dispatcher = NULL;
@@ -545,27 +543,27 @@ kev_multival_t kev_smc_enter(kev_secure_pageno_t disp_page, uintptr_t arg1,
     return ret;
 }
 
-kev_multival_t kev_smc_resume(kev_secure_pageno_t disp_page)
+kom_multival_t kom_smc_resume(kom_secure_pageno_t disp_page)
 {
-    kev_multival_t ret;
+    kom_multival_t ret;
 
     ret.x.val = 0;
     
-    if (!page_is_typed(disp_page, KEV_PAGE_DISPATCHER)) {
-        ret.x.err = KEV_ERR_INVALID_PAGENO;
+    if (!page_is_typed(disp_page, KOM_PAGE_DISPATCHER)) {
+        ret.x.err = KOM_ERR_INVALID_PAGENO;
         return ret;
     }
 
-    struct kev_dispatcher *dispatcher = page_monvaddr(disp_page);
-    struct kev_addrspace *addrspace = g_pagedb[disp_page].addrspace;
+    struct kom_dispatcher *dispatcher = page_monvaddr(disp_page);
+    struct kom_addrspace *addrspace = g_pagedb[disp_page].addrspace;
 
-    if (addrspace->state != KEV_ADDRSPACE_FINAL) {
-        ret.x.err = KEV_ERR_NOT_FINAL;
+    if (addrspace->state != KOM_ADDRSPACE_FINAL) {
+        ret.x.err = KOM_ERR_NOT_FINAL;
         return ret;
     }
 
     if (!dispatcher->entered) {
-        ret.x.err = KEV_ERR_NOT_ENTERED;
+        ret.x.err = KOM_ERR_NOT_ENTERED;
         return ret;
     }
 
@@ -578,7 +576,7 @@ kev_multival_t kev_smc_resume(kev_secure_pageno_t disp_page)
     g_cur_dispatcher = dispatcher;
     ret.raw = dispatch(dispatcher);
     leave_secure_world();
-    if (ret.x.err == KEV_ERR_SUCCESS) {
+    if (ret.x.err == KOM_ERR_SUCCESS) {
         dispatcher->entered = false;
     }
     g_cur_dispatcher = NULL;
@@ -589,62 +587,62 @@ kev_multival_t kev_smc_resume(kev_secure_pageno_t disp_page)
 uint64_t smchandler(uintptr_t callno, uintptr_t arg1, uintptr_t arg2,
                     uintptr_t arg3, uintptr_t arg4)
 {
-    kev_multival_t ret;
+    kom_multival_t ret;
 
     ret.x.val = 0;
 
     switch (callno) {
-    case KEV_SMC_QUERY:
-        ret.x.err = KEV_MAGIC;
+    case KOM_SMC_QUERY:
+        ret.x.err = KOM_MAGIC;
         break;
 
-    case KEV_SMC_GETPHYSPAGES:
-        ret.x.val = kev_smc_get_phys_pages();
-        ret.x.err = KEV_ERR_SUCCESS;
+    case KOM_SMC_GETPHYSPAGES:
+        ret.x.val = kom_smc_get_phys_pages();
+        ret.x.err = KOM_ERR_SUCCESS;
         break;
 
-    case KEV_SMC_INIT_ADDRSPACE:
-        ret.x.err = kev_smc_init_addrspace(arg1, arg2);
+    case KOM_SMC_INIT_ADDRSPACE:
+        ret.x.err = kom_smc_init_addrspace(arg1, arg2);
         break;
 
-    case KEV_SMC_INIT_DISPATCHER:
-        ret.x.err = kev_smc_init_dispatcher(arg1, arg2, arg3);
+    case KOM_SMC_INIT_DISPATCHER:
+        ret.x.err = kom_smc_init_dispatcher(arg1, arg2, arg3);
         break;
 
-    case KEV_SMC_INIT_L2PTABLE:
-        ret.x.err = kev_smc_init_l2table(arg1, arg2, arg3);
+    case KOM_SMC_INIT_L2PTABLE:
+        ret.x.err = kom_smc_init_l2table(arg1, arg2, arg3);
         break;
 
-    case KEV_SMC_MAP_SECURE:
-        ret.x.err = kev_smc_map_secure(arg1, arg2, arg3, arg4);
+    case KOM_SMC_MAP_SECURE:
+        ret.x.err = kom_smc_map_secure(arg1, arg2, arg3, arg4);
         break;
 
-    case KEV_SMC_MAP_INSECURE:
-        ret.x.err = kev_smc_map_insecure(arg1, arg2, arg3);
+    case KOM_SMC_MAP_INSECURE:
+        ret.x.err = kom_smc_map_insecure(arg1, arg2, arg3);
         break;
 
-    case KEV_SMC_REMOVE:
-        ret.x.err = kev_smc_remove(arg1);
+    case KOM_SMC_REMOVE:
+        ret.x.err = kom_smc_remove(arg1);
         break;
     
-    case KEV_SMC_FINALISE:
-        ret.x.err = kev_smc_finalise(arg1);
+    case KOM_SMC_FINALISE:
+        ret.x.err = kom_smc_finalise(arg1);
         break;
 
-    case KEV_SMC_ENTER:
-        ret = kev_smc_enter(arg1, arg2, arg3, arg4);
+    case KOM_SMC_ENTER:
+        ret = kom_smc_enter(arg1, arg2, arg3, arg4);
         break;
 
-    case KEV_SMC_RESUME:
-        ret = kev_smc_resume(arg1);
+    case KOM_SMC_RESUME:
+        ret = kom_smc_resume(arg1);
         break;
 
-    case KEV_SMC_STOP:
-        ret.x.err = kev_smc_stop(arg1);
+    case KOM_SMC_STOP:
+        ret.x.err = kom_smc_stop(arg1);
         break;
 
     default:
-        ret.x.err = KEV_ERR_INVALID;
+        ret.x.err = KOM_ERR_INVALID;
         break;
     }
 
