verified/smcapi.s.dfy
@@ -1,4 +1,4 @@
-include "kev_common.s.dfy"
+include "kom_common.s.dfy"
 include "pagedb.s.dfy"
 
 
@@ -13,14 +13,14 @@ predicate pageIsFree(d:PageDb, pg:PageNr)
 
 predicate physPageIsRam( physPage: int )
 {
-   physPage * KEVLAR_PAGE_SIZE() < SecurePhysBase()
+   physPage * PAGESIZE() < SecurePhysBase()
 }
 
 predicate physPageIsSecure( physPage: int )
 {
-    var paddr := physPage * KEVLAR_PAGE_SIZE();
+    var paddr := physPage * PAGESIZE();
     SecurePhysBase() <= paddr < SecurePhysBase() +
-        KEVLAR_SECURE_NPAGES() * KEVLAR_PAGE_SIZE()
+        KOM_SECURE_NPAGES() * PAGESIZE()
 }
 
 predicate l1indexInUse(d: PageDb, a: PageNr, l1index: int)
@@ -51,7 +51,7 @@ function updateL2Pte(pageDbIn: PageDb, a: PageNr, mapping: Mapping, l2e : L2PTE)
     : PageDb 
     requires validPageDb(pageDbIn)
     requires isAddrspace(pageDbIn, a)
-    requires isValidMappingTarget(pageDbIn, a, mapping) == KEV_ERR_SUCCESS()
+    requires isValidMappingTarget(pageDbIn, a, mapping) == KOM_ERR_SUCCESS()
     requires pageDbIn[a].entry.state.InitState?
 {
     reveal_validPageDb();
@@ -66,63 +66,63 @@ function updateL2Pte(pageDbIn: PageDb, a: PageNr, mapping: Mapping, l2e : L2PTE)
 }
 
 function isValidMappingTarget(d: PageDb, a: PageNr, mapping: Mapping)
-    : int // KEV_ERROR
+    : int // KOM_ERROR
     requires validPageDb(d)
     requires isAddrspace(d, a)
 {
     reveal_validPageDb();
     var addrspace := d[a].entry;
     if(!addrspace.state.InitState?) then
-        KEV_ERR_ALREADY_FINAL()
-    else if(!mapping.perm.r) then KEV_ERR_INVALID_MAPPING()
+        KOM_ERR_ALREADY_FINAL()
+    else if(!mapping.perm.r) then KOM_ERR_INVALID_MAPPING()
     else if(!(0 <= mapping.l1index < NR_L1PTES())
         || !(0 <= mapping.l2index < NR_L2PTES()) ) then
-        KEV_ERR_INVALID_MAPPING()
+        KOM_ERR_INVALID_MAPPING()
     else
         assert validAddrspace(d, a);
         var l1 := d[addrspace.l1ptnr].entry;
         var l1pte := l1.l1pt[mapping.l1index];
-        if(l1pte.Nothing?) then KEV_ERR_INVALID_MAPPING()
-        else KEV_ERR_SUCCESS()
+        if(l1pte.Nothing?) then KOM_ERR_INVALID_MAPPING()
+        else KOM_ERR_SUCCESS()
 }
 
 //============================================================================
 // Behavioral Specification of Monitor Calls
 //=============================================================================
-function smc_query() : int { KEV_MAGIC() }
+function smc_query() : int { KOM_MAGIC() }
 
-function smc_getPhysPages() : int { KEVLAR_SECURE_NPAGES() }
+function smc_getPhysPages() : int { KOM_SECURE_NPAGES() }
 
 function smc_initAddrspace(pageDbIn: PageDb, addrspacePage: PageNr, l1PTPage: PageNr)
-    : (PageDb, int) // PageDbOut, KEV_ERR
+    : (PageDb, int) // PageDbOut, KOM_ERR
     requires validPageDb(pageDbIn);
 {
     reveal_validPageDb();
     var g := pageDbIn;
     if(!validPageNr(addrspacePage) || !validPageNr(l1PTPage) ||
         addrspacePage == l1PTPage) then
-        (pageDbIn, KEV_ERR_INVALID_PAGENO())
+        (pageDbIn, KOM_ERR_INVALID_PAGENO())
     else if(l1PTPage % 4 != 0) then
-        (pageDbIn, KEV_ERR_INVALID_PAGENO())
+        (pageDbIn, KOM_ERR_INVALID_PAGENO())
     else if( !g[addrspacePage].PageDbEntryFree? || !g[l1PTPage].PageDbEntryFree? ) then
-        (pageDbIn, KEV_ERR_PAGEINUSE())
+        (pageDbIn, KOM_ERR_PAGEINUSE())
     else
         var addrspace := Addrspace(l1PTPage, 1, InitState);
         var l1PT := L1PTable(SeqRepeat(NR_L1PTES(),Nothing));
         var pageDbOut := 
             (pageDbIn[addrspacePage := PageDbEntryTyped(addrspacePage, addrspace)])[
                 l1PTPage := PageDbEntryTyped(addrspacePage, l1PT)];
-        (pageDbOut, KEV_ERR_SUCCESS())
+        (pageDbOut, KOM_ERR_SUCCESS())
 }
 
 function smc_initDispatcher(pageDbIn: PageDb, page:PageNr, addrspacePage:PageNr,
     entrypoint:int)
-    : (PageDb, int) // PageDbOut, KEV_ERR
+    : (PageDb, int) // PageDbOut, KOM_ERR
     requires validPageDb(pageDbIn);
 {
     reveal_validPageDb();
    if(!isAddrspace(pageDbIn, addrspacePage)) then
-       (pageDbIn, KEV_ERR_INVALID_ADDRSPACE())
+       (pageDbIn, KOM_ERR_INVALID_ADDRSPACE())
    else
        var ctxt := DispatcherContext(map[], entrypoint,encode_mode(User));
        allocatePage(pageDbIn, page, addrspacePage, Dispatcher(entrypoint, false, ctxt))
@@ -157,9 +157,9 @@ function smc_initL2PTable(pageDbIn: PageDb, page: PageNr,
     requires validPageDb(pageDbIn)
 {
     reveal_validPageDb();
-    if(!(0<= l1index < NR_L1PTES())) then (pageDbIn, KEV_ERR_INVALID_MAPPING())
+    if(!(0<= l1index < NR_L1PTES())) then (pageDbIn, KOM_ERR_INVALID_MAPPING())
     else if(!isAddrspace(pageDbIn, addrspacePage)) then
-        (pageDbIn, KEV_ERR_INVALID_ADDRSPACE())
+        (pageDbIn, KOM_ERR_INVALID_ADDRSPACE())
 
     // This gets caught later in allocatePage, but putting the check
     // here means that the addrspace's state will not be stopped for the
@@ -167,15 +167,15 @@ function smc_initL2PTable(pageDbIn: PageDb, page: PageNr,
     // is actually an l1pt table, which is true as long as the addrspace
     // is not stopped.
     else if(pageDbIn[addrspacePage].entry.state != InitState) then
-        (pageDbIn, KEV_ERR_ALREADY_FINAL())
+        (pageDbIn, KOM_ERR_ALREADY_FINAL())
     else if(l1indexInUse(pageDbIn, addrspacePage, l1index)) then
-        (pageDbIn, KEV_ERR_ADDRINUSE())
+        (pageDbIn, KOM_ERR_ADDRINUSE())
     else 
         var l2pt := L2PTable(SeqRepeat(NR_L2PTES(), NoMapping));
         // allocate the page
         var (pagedb, err) := allocatePage(pageDbIn, page, addrspacePage, l2pt);
         // update the L1 table
-        if err == KEV_ERR_SUCCESS() then
+        if err == KOM_ERR_SUCCESS() then
             var l1ptnr := pagedb[addrspacePage].entry.l1ptnr;
             (installL1PTEInPageDb(pagedb, l1ptnr, page, l1index), err)
         else
@@ -193,30 +193,30 @@ predicate allocatePageEntryValid(entry: PageDbEntryTyped)
 // This is not literally an SMC handler. Move elsewhere in file???
 function allocatePage_inner(pageDbIn: PageDb, securePage: PageNr,
     addrspacePage:PageNr, entry:PageDbEntryTyped)
-    : (PageDb, int) // PageDbOut, KEV_ERR
+    : (PageDb, int) // PageDbOut, KOM_ERR
     requires validPageDb(pageDbIn)
     requires validAddrspacePage(pageDbIn, addrspacePage)
     requires allocatePageEntryValid(entry)
 {
     reveal_validPageDb();
     var addrspace := pageDbIn[addrspacePage].entry;
-    if(!validPageNr(securePage)) then (pageDbIn, KEV_ERR_INVALID_PAGENO())
-    else if(!pageIsFree(pageDbIn, securePage)) then (pageDbIn, KEV_ERR_PAGEINUSE())
+    if(!validPageNr(securePage)) then (pageDbIn, KOM_ERR_INVALID_PAGENO())
+    else if(!pageIsFree(pageDbIn, securePage)) then (pageDbIn, KOM_ERR_PAGEINUSE())
     else if(addrspace.state != InitState) then
-        (pageDbIn,KEV_ERR_ALREADY_FINAL())
+        (pageDbIn,KOM_ERR_ALREADY_FINAL())
     // TODO ?? Model page clearing for non-data pages?
     else
         var updatedAddrspace := addrspace.(refcount := addrspace.refcount + 1);
         var pageDbOut := (pageDbIn[
             securePage := PageDbEntryTyped(addrspacePage, entry)])[
             addrspacePage := pageDbIn[addrspacePage].(entry := updatedAddrspace)];
-        (pageDbOut, KEV_ERR_SUCCESS())
+        (pageDbOut, KOM_ERR_SUCCESS())
 }
 
 // TODO move this elsewhere since it is not a monitor call
 function allocatePage(pageDbIn: PageDb, securePage: PageNr,
     addrspacePage:PageNr, entry:PageDbEntryTyped )
-    : (PageDb, int) // PageDbOut, KEV_ERR
+    : (PageDb, int) // PageDbOut, KOM_ERR
     requires validPageDb(pageDbIn)
     requires validAddrspacePage(pageDbIn, addrspacePage)
     requires allocatePageEntryValid(entry)
@@ -228,59 +228,59 @@ function allocatePage(pageDbIn: PageDb, securePage: PageNr,
 }
 
 function smc_remove(pageDbIn: PageDb, page: PageNr)
-    : (PageDb, int) // PageDbOut, KEV_ERR
+    : (PageDb, int) // PageDbOut, KOM_ERR
     requires validPageDb(pageDbIn)
 {
     reveal_validPageDb();
     if(!validPageNr(page)) then
-        (pageDbIn, KEV_ERR_INVALID_PAGENO())
+        (pageDbIn, KOM_ERR_INVALID_PAGENO())
     else if(pageDbIn[page].PageDbEntryFree?) then
-        (pageDbIn, KEV_ERR_SUCCESS())
+        (pageDbIn, KOM_ERR_SUCCESS())
     else 
         var e := pageDbIn[page].entry;
         var addrspacePage := pageDbIn[page].addrspace;
         var addrspace := pageDbIn[addrspacePage].entry;
         if( e.Addrspace? ) then
-           if(e.refcount !=0) then (pageDbIn, KEV_ERR_PAGEINUSE())
-           else (pageDbIn[page := PageDbEntryFree], KEV_ERR_SUCCESS())
+           if(e.refcount !=0) then (pageDbIn, KOM_ERR_PAGEINUSE())
+           else (pageDbIn[page := PageDbEntryFree], KOM_ERR_SUCCESS())
         else 
             if( !addrspace.state.StoppedState?) then
-                (pageDbIn, KEV_ERR_NOT_STOPPED())
+                (pageDbIn, KOM_ERR_NOT_STOPPED())
             else 
                 assert page in addrspaceRefs(pageDbIn, addrspacePage);
                 var updatedAddrspace := match addrspace
                     case Addrspace(l1, ref, state) => Addrspace(l1, ref - 1, state);
                 var pageDbOut := (pageDbIn[page := PageDbEntryFree])[
                     addrspacePage := PageDbEntryTyped(addrspacePage, updatedAddrspace)];
-                (pageDbOut, KEV_ERR_SUCCESS())
+                (pageDbOut, KOM_ERR_SUCCESS())
 }
 
 function smc_mapSecure(pageDbIn: PageDb, page: PageNr, addrspacePage: PageNr,
-    mapping: Mapping, physPage: int) : (PageDb, int) // PageDbOut, KEV_ERR
+    mapping: Mapping, physPage: int) : (PageDb, int) // PageDbOut, KOM_ERR
     requires validPageDb(pageDbIn)
 {
     reveal_validPageDb();
     if(!isAddrspace(pageDbIn, addrspacePage)) then
-        (pageDbIn, KEV_ERR_INVALID_ADDRSPACE())
+        (pageDbIn, KOM_ERR_INVALID_ADDRSPACE())
     else 
         var err := isValidMappingTarget(pageDbIn, addrspacePage, mapping);
-        if( err != KEV_ERR_SUCCESS() ) then (pageDbIn, err)
+        if( err != KOM_ERR_SUCCESS() ) then (pageDbIn, err)
         else 
             // I'm not actually sure if this makes sense. I don't know
             // that physPage is actually modeling a physical page here...
             // address translation isn't modeled here at all.
             if( physPageInvalid(physPage) ) then
-                (pageDbIn, KEV_ERR_INVALID_PAGENO())
+                (pageDbIn, KOM_ERR_INVALID_PAGENO())
             else
                 var ap_ret := allocatePage(pageDbIn, page,
                     addrspacePage, DataPage);
                 var pageDbA := ap_ret.0;
                 var errA := ap_ret.1;
-                if(errA != KEV_ERR_SUCCESS()) then (pageDbIn, errA)
+                if(errA != KOM_ERR_SUCCESS()) then (pageDbIn, errA)
                 else
                     var l2pte := SecureMapping(page, mapping.perm.w, mapping.perm.x);
                     var pageDbOut := updateL2Pte(pageDbA, addrspacePage, mapping, l2pte);
-                    (pageDbOut, KEV_ERR_SUCCESS())
+                    (pageDbOut, KOM_ERR_SUCCESS())
 }
 
 function smc_mapInsecure(pageDbIn: PageDb, addrspacePage: PageNr,
@@ -289,18 +289,18 @@ function smc_mapInsecure(pageDbIn: PageDb, addrspacePage: PageNr,
 {
     reveal_validPageDb();
     if(!isAddrspace(pageDbIn, addrspacePage)) then
-        (pageDbIn, KEV_ERR_INVALID_ADDRSPACE())
+        (pageDbIn, KOM_ERR_INVALID_ADDRSPACE())
     else
         var err := isValidMappingTarget(pageDbIn, addrspacePage, mapping);
-        if( err != KEV_ERR_SUCCESS() ) then (pageDbIn, err)
+        if( err != KOM_ERR_SUCCESS() ) then (pageDbIn, err)
         else if( physPage < 0
-            || physPage >= KEVLAR_PHYSMEM_LIMIT() / KEVLAR_PAGE_SIZE()
+            || physPage >= KOM_PHYSMEM_LIMIT() / PAGESIZE()
             || physPageIsSecure(physPage) ) then
-            (pageDbIn, KEV_ERR_INVALID_PAGENO())
+            (pageDbIn, KOM_ERR_INVALID_PAGENO())
         else
             var l2pte := InsecureMapping( physPage,  mapping.perm.w);
             var pageDbOut := updateL2Pte(pageDbIn, addrspacePage, mapping, l2pte);
-            (pageDbOut, KEV_ERR_SUCCESS())
+            (pageDbOut, KOM_ERR_SUCCESS())
 }
 
 function smc_finalise(pageDbIn: PageDb, addrspacePage: PageNr) : (PageDb, int)
@@ -308,16 +308,16 @@ function smc_finalise(pageDbIn: PageDb, addrspacePage: PageNr) : (PageDb, int)
 {
     reveal_validPageDb();
     if(!isAddrspace(pageDbIn, addrspacePage)) then
-        (pageDbIn, KEV_ERR_INVALID_ADDRSPACE())
+        (pageDbIn, KOM_ERR_INVALID_ADDRSPACE())
     else if(pageDbIn[addrspacePage].entry.state != InitState) then
-        (pageDbIn, KEV_ERR_ALREADY_FINAL())
+        (pageDbIn, KOM_ERR_ALREADY_FINAL())
     else
         var addrspace := pageDbIn[addrspacePage].entry;
         var updatedAddrspace := match addrspace
             case Addrspace(l1, ref, state) => Addrspace(l1, ref, FinalState);
         var pageDbOut := pageDbIn[
             addrspacePage := PageDbEntryTyped(addrspacePage, updatedAddrspace)];
-        (pageDbOut, KEV_ERR_SUCCESS())
+        (pageDbOut, KOM_ERR_SUCCESS())
 }
 
 function smc_enter(pageDbIn: PageDb, dispPage: PageNr, arg1: int, arg2: int, arg3: int)
@@ -327,13 +327,13 @@ function smc_enter(pageDbIn: PageDb, dispPage: PageNr, arg1: int, arg2: int, arg
     reveal_validPageDb();
     var d := pageDbIn; var p := dispPage;
     if(!(validPageNr(p) && d[p].PageDbEntryTyped? && d[p].entry.Dispatcher?)) then
-        (pageDbIn, KEV_ERR_INVALID_PAGENO())
+        (pageDbIn, KOM_ERR_INVALID_PAGENO())
     else if(var a := d[p].addrspace; d[a].entry.state != FinalState) then
-        (pageDbIn, KEV_ERR_NOT_FINAL())
+        (pageDbIn, KOM_ERR_NOT_FINAL())
     else if(d[p].entry.entered) then
-        (pageDbIn, KEV_ERR_ALREADY_ENTERED())
+        (pageDbIn, KOM_ERR_ALREADY_ENTERED())
     else
-        (pageDbIn, KEV_ERR_SUCCESS())
+        (pageDbIn, KOM_ERR_SUCCESS())
 }
 
 function smc_resume(pageDbIn: PageDb, dispPage: PageNr)
@@ -343,13 +343,13 @@ function smc_resume(pageDbIn: PageDb, dispPage: PageNr)
     reveal_validPageDb();
     var d := pageDbIn; var p := dispPage;
     if(!(validPageNr(p) && d[p].PageDbEntryTyped? && d[p].entry.Dispatcher?)) then
-        (pageDbIn, KEV_ERR_INVALID_PAGENO())
+        (pageDbIn, KOM_ERR_INVALID_PAGENO())
     else if(var a := d[p].addrspace; d[a].entry.state != FinalState) then
-        (pageDbIn, KEV_ERR_NOT_FINAL())
+        (pageDbIn, KOM_ERR_NOT_FINAL())
     else if(!d[p].entry.entered) then
-        (pageDbIn, KEV_ERR_NOT_ENTERED())
+        (pageDbIn, KOM_ERR_NOT_ENTERED())
     else
-        (pageDbIn, KEV_ERR_SUCCESS())
+        (pageDbIn, KOM_ERR_SUCCESS())
 }
 
 function smc_stop(pageDbIn: PageDb, addrspacePage: PageNr)
@@ -358,16 +358,16 @@ function smc_stop(pageDbIn: PageDb, addrspacePage: PageNr)
 {
     reveal_validPageDb();
     if(!isAddrspace(pageDbIn, addrspacePage)) then
-        (pageDbIn, KEV_ERR_INVALID_ADDRSPACE())
+        (pageDbIn, KOM_ERR_INVALID_ADDRSPACE())
     // else if(pageDbIn[addrspacePage].entry.state == InitState) then
-    //     (pageDbIn, KEV_ERR_ALREADY_FINAL())
+    //     (pageDbIn, KOM_ERR_ALREADY_FINAL())
     else
         var addrspace := pageDbIn[addrspacePage].entry;
         var updatedAddrspace := match addrspace
             case Addrspace(l1, ref, state) => Addrspace(l1, ref, StoppedState);
         var pageDbOut := pageDbIn[
             addrspacePage := PageDbEntryTyped(addrspacePage, updatedAddrspace)];
-        (pageDbOut, KEV_ERR_SUCCESS())
+        (pageDbOut, KOM_ERR_SUCCESS())
 }
 
 //=============================================================================
@@ -378,40 +378,40 @@ function smchandler(pageDbIn: PageDb, callno: int, arg1: int, arg2: int,
     requires validPageDb(pageDbIn)
 {
     reveal_validPageDb();
-    if(callno == KEV_SMC_QUERY()) then (pageDbIn, KEV_MAGIC(), 0)
-    else if(callno == KEV_SMC_GETPHYSPAGES()) then
-        (pageDbIn, KEV_ERR_SUCCESS(), KEVLAR_SECURE_NPAGES())
-    else if(callno == KEV_SMC_INIT_ADDRSPACE()) then
+    if(callno == KOM_SMC_QUERY()) then (pageDbIn, KOM_MAGIC(), 0)
+    else if(callno == KOM_SMC_GETPHYSPAGES()) then
+        (pageDbIn, KOM_ERR_SUCCESS(), KOM_SECURE_NPAGES())
+    else if(callno == KOM_SMC_INIT_ADDRSPACE()) then
         var ret := smc_initAddrspace(pageDbIn, arg1, arg2);
         (ret.0, ret.1, 0)
-    else if(callno == KEV_SMC_INIT_DISPATCHER()) then
+    else if(callno == KOM_SMC_INIT_DISPATCHER()) then
         var ret := smc_initDispatcher(pageDbIn, arg1, arg2, arg3);
         (ret.0, ret.1, 0)
-    else if(callno == KEV_SMC_INIT_L2PTABLE()) then
+    else if(callno == KOM_SMC_INIT_L2PTABLE()) then
         var ret := smc_initL2PTable(pageDbIn, arg1, arg2, arg3);
         (ret.0, ret.1, 0)
-    else if(callno == KEV_SMC_MAP_SECURE()) then
+    else if(callno == KOM_SMC_MAP_SECURE()) then
         var ret := smc_mapSecure(pageDbIn, arg1, arg2, intToMapping(arg3), arg4);
         (ret.0, ret.1, 0)
-    else if(callno == KEV_SMC_MAP_INSECURE()) then
+    else if(callno == KOM_SMC_MAP_INSECURE()) then
         var ret := smc_mapInsecure(pageDbIn, arg1, arg2, intToMapping(arg3));
         (ret.0, ret.1, 0)
-    else if(callno == KEV_SMC_REMOVE()) then
+    else if(callno == KOM_SMC_REMOVE()) then
         var ret := smc_remove(pageDbIn, arg1);
         (ret.0, ret.1, 0)
-    else if(callno == KEV_SMC_FINALISE()) then
+    else if(callno == KOM_SMC_FINALISE()) then
         var ret := smc_finalise(pageDbIn, arg1);
         (ret.0, ret.1, 0)
-    else if(callno == KEV_SMC_ENTER()) then
+    else if(callno == KOM_SMC_ENTER()) then
         var ret := smc_enter(pageDbIn, arg1, arg2, arg3, arg4);
         (ret.0, ret.1, 0)
-    else if(callno == KEV_SMC_RESUME()) then
+    else if(callno == KOM_SMC_RESUME()) then
         var ret := smc_resume(pageDbIn, arg1);
         (ret.0, ret.1, 0)
-    else if(callno == KEV_SMC_STOP()) then
+    else if(callno == KOM_SMC_STOP()) then
         var ret := smc_stop(pageDbIn, arg1);
         (ret.0, ret.1, 0)
-    else (pageDbIn, KEV_ERR_INVALID(), 0)
+    else (pageDbIn, KOM_ERR_INVALID(), 0)
 }
 
 /* Invariant across SMC handler state */
@@ -450,7 +450,7 @@ lemma allocatePagePreservesPageDBValidity(pageDbIn: PageDb,
     var pageDbOut := result.0;
     var errOut := result.1;
 
-    if ( errOut != KEV_ERR_SUCCESS() ){
+    if ( errOut != KOM_ERR_SUCCESS() ){
         // The error case is trivial because PageDbOut == PageDbIn
     } else {
         forall () ensures validPageDbEntry(pageDbOut, addrspacePage);
