verified/kom_common.s.dfy
@@ -1,0 +1,145 @@
+include "ARMdef.dfy"
+
+function method KOM_MAGIC():int { 0x4b6d646f }
+
+//-----------------------------------------------------------------------------
+// SMC Call Numbers
+//-----------------------------------------------------------------------------
+function method KOM_SMC_QUERY():int           { 1  }
+function method KOM_SMC_GETPHYSPAGES():int    { 2  }
+function method KOM_SMC_INIT_ADDRSPACE():int  { 10 }
+function method KOM_SMC_INIT_DISPATCHER():int { 11 }
+function method KOM_SMC_INIT_L2PTABLE():int   { 12 }
+function method KOM_SMC_MAP_SECURE():int      { 13 }
+function method KOM_SMC_MAP_INSECURE():int    { 14 }
+function method KOM_SMC_REMOVE():int          { 20 }
+function method KOM_SMC_FINALISE():int        { 21 }
+function method KOM_SMC_ENTER():int           { 22 }
+function method KOM_SMC_RESUME():int          { 23 }
+function method KOM_SMC_STOP():int            { 29 }
+
+//-----------------------------------------------------------------------------
+// Errors
+//-----------------------------------------------------------------------------
+function method KOM_ERR_SUCCESS():int
+    ensures KOM_ERR_SUCCESS() == 0;
+    { 0 }
+function method KOM_ERR_INVALID_PAGENO():int     { 1  }
+function method KOM_ERR_PAGEINUSE():int          { 2  }
+function method KOM_ERR_INVALID_ADDRSPACE():int  { 3  }
+function method KOM_ERR_ALREADY_FINAL():int      { 4  }
+function method KOM_ERR_NOT_FINAL():int          { 5  }
+function method KOM_ERR_INVALID_MAPPING():int    { 6  }
+function method KOM_ERR_ADDRINUSE():int          { 7  }
+function method KOM_ERR_NOT_STOPPED():int        { 8  }
+function method KOM_ERR_INTERRUPTED():int        { 9  }
+function method KOM_ERR_FAULT():int              { 10 }
+function method KOM_ERR_ALREADY_ENTERED():int    { 11 }
+function method KOM_ERR_NOT_ENTERED():int        { 12 }
+function method KOM_ERR_INVALID():int            { 0x1_0000_0000 }
+
+//-----------------------------------------------------------------------------
+// Memory Regions
+//-----------------------------------------------------------------------------
+function method KOM_MON_VBASE():mem
+    ensures KOM_MON_VBASE() == 0x4000_0000;
+    { 0x4000_0000 }
+function method KOM_DIRECTMAP_VBASE():mem
+    ensures KOM_DIRECTMAP_VBASE() == 0x8000_0000;
+    { 0x8000_0000 }
+function method KOM_DIRECTMAP_SIZE():word   { 0x8000_0000 }
+function method KOM_SECURE_RESERVE():mem
+    ensures KOM_SECURE_RESERVE() == 1 * 1024 * 1024;
+    { 1 * 1024 * 1024 }
+function method KOM_SECURE_NPAGES():word
+    ensures KOM_SECURE_NPAGES() == 256;
+    { KOM_SECURE_RESERVE() / PAGESIZE() }
+
+// we don't support/consider more than 1GB of physical memory in our maps
+function method KOM_PHYSMEM_LIMIT():mem
+    { 0x4000_0000 }
+
+function KOM_STACK_SIZE():mem
+    { 0x4000 }
+
+// we don't know where the stack is exactly, but we know how big it is
+function {:axiom} StackLimit():mem
+    ensures KOM_MON_VBASE() <= StackLimit()
+    ensures StackLimit() <= KOM_DIRECTMAP_VBASE() - KOM_STACK_SIZE()
+
+function StackBase():mem
+{
+    StackLimit() + KOM_STACK_SIZE()
+}
+
+predicate address_is_secure(m:mem)
+{
+    (KOM_DIRECTMAP_VBASE() + SecurePhysBase()) <= m <
+        (KOM_DIRECTMAP_VBASE() + SecurePhysBase() + KOM_SECURE_RESERVE())
+}        
+
+//-----------------------------------------------------------------------------
+// Globals
+//-----------------------------------------------------------------------------
+
+function method PAGEDB_ENTRY_SIZE():int { 8 }
+function method G_PAGEDB_SIZE():int
+    ensures G_PAGEDB_SIZE() == KOM_SECURE_NPAGES() * PAGEDB_ENTRY_SIZE();
+    { KOM_SECURE_NPAGES() * PAGEDB_ENTRY_SIZE() }
+
+function method {:opaque} CurAddrspaceOp(): operand { OSymbol("g_cur_addrspace") }
+function method {:opaque} PageDb(): operand { OSymbol("g_pagedb") }
+function method {:opaque} SecurePhysBaseOp(): operand { OSymbol("g_secure_physbase") }
+
+// the phys base is unknown, but never changes
+function {:axiom} SecurePhysBase(): mem
+    ensures 0 < SecurePhysBase() <= KOM_PHYSMEM_LIMIT() - KOM_SECURE_RESERVE();
+    ensures PageAligned(SecurePhysBase());
+
+function method KomGlobalDecls(): globaldecls
+    ensures ValidGlobalDecls(KomGlobalDecls());
+{
+    reveal_PageDb(); reveal_SecurePhysBaseOp(); reveal_CurAddrspaceOp();
+    map[SecurePhysBaseOp() := 4, //BytesPerWord() 
+        CurAddrspaceOp() := 4,  //BytesPerWord()
+        PageDb() := G_PAGEDB_SIZE()]
+}
+
+//-----------------------------------------------------------------------------
+// Application-level state invariants
+//
+// These are part of the spec, since we rely on the bootloader setting
+// up our execution environment so they are ensured on SMC handler entry.
+//-----------------------------------------------------------------------------
+
+predicate ValidStack(s:state)
+    requires ValidState(s)
+{
+    WordAligned(OperandContents(s, OSP))
+    && StackLimit() < OperandContents(s, OSP) <= StackBase()
+}
+
+predicate SaneMem(s:memstate)
+{
+    ValidMemState(s)
+    // TODO: our insecure phys mapping must be valid
+    //&& ValidMemRange(KOM_DIRECTMAP_VBASE(),
+    //    (KOM_DIRECTMAP_VBASE() + MonitorPhysBaseValue()))
+    // our secure phys mapping must be valid
+    && ValidMemRange(KOM_DIRECTMAP_VBASE() + SecurePhysBase(),
+        (KOM_DIRECTMAP_VBASE() + SecurePhysBase() + KOM_SECURE_RESERVE()))
+    // the stack must be mapped
+    && ValidMemRange(StackLimit(), StackBase())
+    // globals are as we expect
+    && KomGlobalDecls() == TheGlobalDecls()
+    && GlobalFullContents(s, SecurePhysBaseOp()) == [SecurePhysBase()]
+    // XXX: workaround so dafny sees that these are distinct
+    && SecurePhysBaseOp() != PageDb()
+    && SecurePhysBaseOp() != CurAddrspaceOp()
+    && CurAddrspaceOp() != PageDb()
+}
+
+predicate SaneState(s:state)
+{
+    ValidState(s) && ValidStack(s) && SaneMem(s.m) && mode_of_state(s) == Monitor
+}
