README.md
@@ -1,17 +1,17 @@
-Project Kevlar
+Project Komodo
 ==============
 
 Components
 ----------
 
-Kevlar consists of a number of different components:
+Komodo consists of a number of different components:
 
  1. A minimal Raspberry Pi bootloader (`piloader`) which loads the
     monitor in secure world, and then boots an existing OS image
     (typically Linux) in normal world.
  
  2. A secure-world monitor program (`monitor`) which implements the
-    Kevlar protection model. This will be replaced with verified code.
+    Komodo protection model. This will be replaced with verified code.
  
  3. A Linux kernel driver (`driver`) which interacts with the monitor
     using secure monitor calls (SMCs), and implements an `ioctl`
@@ -19,21 +19,20 @@ Kevlar consists of a number of different components:
     regions.
 
 The loader, monitor and kernel are all linked together into a single
-bootable image (`piimage/kevlar.img`).
+bootable image (`piimage/piimage.img`).
 
 Building
 --------
 
-Kevlar builds on a Linux-like environment, including Cygwin and WSL.
+Komodo builds on a Linux-like environment, including Cygwin and WSL.
 
 Required tools:
  * GNU make
- 
+
  * An ARM EABI cross-compiler (gcc and binutils), such as [this Linaro
    toolchain](http://releases.linaro.org/components/toolchain/binaries/4.9-2016.02/arm-eabi/)
-   
- * To build the verified code, Dafny and Spartan executables, built from [the impsec branch of the
-   GitHubWIP Ironclad repository](https://msresearch.visualstudio.com/Ironclad/_git/GitHubWIP?path=%2Fimpsec&version=GBimpsec&_a=contents)
+
+ * To build the verified code, Dafny and Spartan executables, built from [XXX: missing link](TODO)
 
  * To build the Linux driver, see
    [here](https://www.raspberrypi.org/documentation/linux/kernel/building.md)
@@ -41,6 +40,4 @@ Required tools:
 
 The supported platform is currently Raspberry Pi 2, either a real
 board, or a custom QEMU, available from [this GitHub
-branch](https://github.com/0xabu/qemu/commits/raspi-tzkludges). If
-you're at MSR, you can also find precompiled Windows binaries at
-[\\\\research\root\public\kevlar\qemu](file:////research/root/public/kevlar/qemu).
+branch](https://github.com/0xabu/qemu/commits/raspi-tzkludges).
