piimage/subdir.mk
@@ -1,18 +1,18 @@
-PIIMAGE_LINKER_SCRIPT := $(dir)/kevlar.lds
+PIIMAGE_LINKER_SCRIPT := $(dir)/piimage.lds
 PIIMAGE_ELF_INPUTS := piloader/piloader.elf $(dir)/kernelblob.elf monitor/monitor.elf
 
 $(dir)/kernelblob.elf: $(GUEST_KERNEL)
 	$(OBJCOPY) -I binary -O elf32-littlearm -B arm $< $@
 
-$(dir)/kevlar.elf: $(PIIMAGE_ELF_INPUTS) $(PIIMAGE_LINKER_SCRIPT)
+$(dir)/piimage.elf: $(PIIMAGE_ELF_INPUTS) $(PIIMAGE_LINKER_SCRIPT)
 	$(LD) $(LDFLAGS_ALL) -T $(PIIMAGE_LINKER_SCRIPT) -o $@ $(PIIMAGE_ELF_INPUTS) -z muldefs
 
-$(dir)/kevlar.img: $(dir)/kevlar.elf
+$(dir)/piimage.img: $(dir)/piimage.elf
 	$(OBJCOPY) $< -O binary $@
 
-CLEAN := $(CLEAN) $(dir)/kevlar.elf $(dir)/kevlar.img
+CLEAN := $(CLEAN) $(dir)/kernelblob.elf $(dir)/piimage.elf $(dir)/piimage.img
 
 .PHONY: install
 
-install:: $(dir)/kevlar.img $(dir)/config.txt
+install:: $(TARGET) $(dir)/config.txt
 	cp -uv $^ $(INSTALLDIR)
